More agility in Blake2S

code/blake2/Hacl.Impl.Blake2s.fst
@@ -14,16 +14,21 @@ module Seq = Lib.Sequence
 module Loops = Lib.LoopCombinators
 module Spec = Spec.Blake2
 
+(* Alias types from Specification *)
+type alg = Spec.alg
+type word_t a = Spec.word_t a
+type limb_t a = Spec.limb_t a
 
 (* Define algorithm parameters *)
-type vector_wp = lbuffer uint32 Spec.size_block_w
-type block_wp = lbuffer uint32 Spec.size_block_w
-type block_p = lbuffer uint8 (Spec.size_block Spec.Blake2S)
-type hash_wp = lbuffer uint32 Spec.size_hash_w
+type vector_wp (a:alg) = lbuffer (word_t a) Spec.size_block_w
+type block_wp (a:alg) = lbuffer (word_t a) Spec.size_block_w
+type block_p (a:alg) = lbuffer uint8 (Spec.size_block a)
+type hash_wp (a:alg) = lbuffer (word_t a) Spec.size_hash_w
 type index_t = n:size_t{size_v n < 16}
 
-inline_for_extraction let size_word : size_t = size 4
-inline_for_extraction let size_block x : n:size_t{v n > 0 /\ v n == Spec.size_block Spec.Blake2.Blake2S} = (size Spec.size_block_w) *. size_word
+inline_for_extraction let size_word (a:alg) = size (Spec.size_word a)
+inline_for_extraction let size_block (a:alg) : n:size_t{v n > 0 /\ v n == Spec.size_block a} =
+  (size Spec.size_block_w) *. (size_word a)
 
 
 /// Constants
@@ -35,31 +40,32 @@ let rTable_S = icreateL_global Spec.rTable_list_S
 /// Accessors for constants
 
 val get_iv:
-  s:size_t{size_v s < 8} ->
-  Stack uint32
+    p:alg
+  -> s:size_t{size_v s < 8} ->
+  Stack (word_t p)
     (requires (fun h -> True))
     (ensures  (fun h0 z h1 -> h0 == h1 /\
-      uint_v z == uint_v (Seq.index (Spec.ivTable Spec.Blake2S) (size_v s))))
+      uint_v z == uint_v (Seq.index (Spec.ivTable p) (size_v s))))
 
 [@ Substitute ]
-let get_iv s =
-  recall_contents const_iv (Spec.ivTable Spec.Blake2S);
-  let r : size_t = iindex const_iv s in
+let get_iv p s =
+  recall_contents const_iv (Spec.ivTable p);
+  let r = iindex const_iv s in
   secret r
-
 
 
 #set-options "--z3rlimit 50"
 [@ Substitute ]
 val set_iv:
-  hash:hash_wp ->
+    p:alg
+  -> hash:hash_wp p ->
   Stack unit
     (requires (fun h -> live h hash))
     (ensures  (fun h0 _ h1 -> modifies1 hash h0 h1
-                         /\ h1.[hash] == Seq.map secret (Spec.ivTable Spec.Blake2S)))
+                         /\ h1.[hash] == Seq.map secret (Spec.ivTable p)))
 [@ Substitute ]
-let set_iv hash =
-  recall_contents const_iv (Spec.ivTable Spec.Blake2S);
+let set_iv a hash =
+  recall_contents const_iv (Spec.ivTable a);
   let h0 = ST.get() in
   imapT hash (size (Spec.size_hash_w)) secret const_iv
 
@@ -67,24 +73,25 @@ let set_iv hash =
 #set-options "--z3rlimit 15"
 
 val set_iv_sub:
-  b:lbuffer uint32 16 ->
+    p:alg
+  -> b:lbuffer (word_t p) 16 ->
   Stack unit
     (requires (fun h -> live h b))
     (ensures  (fun h0 _ h1 -> modifies1 b h0 h1
-                      /\ (let b0: Seq.lseq uint32 16 = h0.[b] in
-                         let b1: Seq.lseq uint32 16 = h1.[b] in
-                         let src = Seq.map secret (Spec.ivTable Spec.Blake2S) in
-                         b1 == Seq.update_sub #uint32 #16 b0 8 8 src)))
+                      /\ (let b0: Seq.lseq (word_t p) 16 = h0.[b] in
+                         let b1: Seq.lseq (word_t p) 16 = h1.[b] in
+                         let src = Seq.map secret (Spec.ivTable p) in
+                         b1 == Seq.update_sub #(word_t p) #16 b0 8 8 src)))
 [@ Substitute ]
-let set_iv_sub b =
+let set_iv_sub p b =
   let h0 = ST.get () in
-  let half0 = sub #uint32 #16 #8 b (size 0) (size 8) in
-  let half1 = sub #uint32 #16 #8 b (size 8) (size 8) in
+  let half0 = sub #(word_t p) #16 #8 b (size 0) (size 8) in
+  let half1 = sub #(word_t p) #16 #8 b (size 8) (size 8) in
   let h1 = ST.get () in
-  set_iv half1;
+  set_iv p half1;
   let h2 = ST.get () in
-  Seq.eq_intro h2.[b] (Seq.concat #uint32 #8 #8 h2.[half0] h2.[half1]);
-  Seq.eq_intro h2.[b] (Seq.update_sub #uint32 #16 h0.[b] 8 8 (Seq.map secret (Spec.ivTable Spec.Blake2S)))
+  Seq.eq_intro h2.[b] (Seq.concat #(word_t p) #8 #8 h2.[half0] h2.[half1]);
+  Seq.eq_intro h2.[b] (Seq.update_sub #(word_t p) #16 h0.[b] 8 8 (Seq.map secret (Spec.ivTable p)))
 
 
 #reset-options
@@ -117,75 +124,76 @@ let get_sigma_sub start i = get_sigma (start +. i)
 #reset-options
 
 val get_r:
-  s:size_t{size_v s < 4} ->
+    p:alg
+  -> s:size_t{size_v s < 4} ->
   Stack (rotval U32)
     (requires (fun h -> True))
-    (ensures  (fun h0 z h1 -> h0 == h1 /\ v z == v (Seq.index (Spec.rTable Spec.Blake2S) (v s))))
+    (ensures  (fun h0 z h1 -> h0 == h1 /\ v z == v (Seq.index (Spec.rTable p) (v s))))
 
 [@ Substitute ]
-let get_r s =
+let get_r a s =
   recall_contents rTable_S (Spec.rTable Spec.Blake2S);
   iindex rTable_S s
 
 
 /// Define algorithm functions
 
-val g1: wv:vector_wp -> a:index_t -> b:index_t -> r:rotval U32 ->
+val g1: p:alg -> wv:vector_wp p -> a:index_t -> b:index_t -> r:rotval U32 ->
   Stack unit
     (requires (fun h -> live h wv))
     (ensures  (fun h0 _ h1 -> modifies1 wv h0 h1
-                         /\ h1.[wv] == Spec.g1 Spec.Blake2S h0.[wv] (v a) (v b) r))
+                         /\ h1.[wv] == Spec.g1 p h0.[wv] (v a) (v b) r))
 
-let g1 wv a b r =
+let g1 al wv a b r =
   let wv_a = wv.(a) in
   let wv_b = wv.(b) in
   wv.(a) <- (wv_a ^. wv_b) >>>. r
 
 
-val g2: wv:vector_wp -> a:index_t -> b:index_t -> x:uint32 ->
+val g2: p:alg -> wv:vector_wp p -> a:index_t -> b:index_t -> x:uint32 ->
   Stack unit
     (requires (fun h -> live h wv))
     (ensures  (fun h0 _ h1 -> modifies1 wv h0 h1
-                         /\ h1.[wv] == Spec.g2 Spec.Blake2S h0.[wv] (v a) (v b) x))
+                         /\ h1.[wv] == Spec.g2 p h0.[wv] (v a) (v b) x))
 
-let g2 wv a b x =
+let g2 al wv a b x =
   let wv_a = wv.(a) in
   let wv_b = wv.(b) in
   wv.(a) <- add_mod #U32 (wv_a +. wv_b) x
 
 
-val blake2_mixing : wv:vector_wp -> a:index_t -> b:index_t -> c:index_t -> d:index_t -> x:uint32 -> y:uint32 ->
+val blake2_mixing : p:alg -> wv:vector_wp p -> a:index_t -> b:index_t -> c:index_t -> d:index_t -> x:word_t p -> y:word_t p ->
   Stack unit
     (requires (fun h -> live h wv))
     (ensures  (fun h0 _ h1 -> modifies1 wv h0 h1
-                         /\ h1.[wv] == Spec.blake2_mixing Spec.Blake2S h0.[wv] (v a) (v b) (v c) (v d) x y))
+                         /\ h1.[wv] == Spec.blake2_mixing p h0.[wv] (v a) (v b) (v c) (v d) x y))
 
-let blake2_mixing wv a b c d x y =
-  let r0 = get_r (size 0) in
-  let r1 = get_r (size 1) in
-  let r2 = get_r (size 2) in
-  let r3 = get_r (size 3) in
-  g2 wv a b x;
-  g1 wv d a r0;
-  g2 wv c d (u32 0);
-  g1 wv b c r1;
-  g2 wv a b y;
-  g1 wv d a r2;
-  g2 wv c d (u32 0);
-  g1 wv b c r3
+let blake2_mixing p wv a b c d x y =
+  let r0 = get_r p (size 0) in
+  let r1 = get_r p (size 1) in
+  let r2 = get_r p (size 2) in
+  let r3 = get_r p (size 3) in
+  g2 p wv a b x;
+  g1 p wv d a r0;
+  g2 p wv c d (u32 0);
+  g1 p wv b c r1;
+  g2 p wv a b y;
+  g1 p wv d a r2;
+  g2 p wv c d (u32 0);
+  g1 p wv b c r3
 
 
 #set-options "--z3rlimit 15"
 
-val blake2_round1 : wv:vector_wp -> m:block_wp -> i:size_t{size_v i <= 9} ->
+val blake2_round1 : p:alg -> wv:vector_wp p -> m:block_wp p -> i:size_t{size_v i <= 9} ->
   Stack unit
     (requires (fun h -> live h wv /\ live h m
                   /\ disjoint wv m))
     (ensures  (fun h0 _ h1 -> modifies1 wv h0 h1
-                         /\ h1.[wv] == Spec.blake2_round1 Spec.Blake2S h0.[wv] h0.[m] (v i)))
+                         /\ h1.[wv] == Spec.blake2_round1 p h0.[wv] h0.[m] (v i)))
 
 [@ Substitute ]
-let blake2_round1 wv m i =
+let blake2_round1 p wv m i =
   let start_idx = (i %. (size 10)) *. (size 16) in
   let s0 = get_sigma_sub start_idx (size 0) in
   let s1 = get_sigma_sub start_idx (size 1) in
@@ -195,23 +203,23 @@ let blake2_round1 wv m i =
   let s5 = get_sigma_sub start_idx (size 5) in
   let s6 = get_sigma_sub start_idx (size 6) in
   let s7 = get_sigma_sub start_idx (size 7) in
-  blake2_mixing wv (size 0) (size 4) (size  8) (size 12) m.(s0) m.(s1);
-  blake2_mixing wv (size 1) (size 5) (size  9) (size 13) m.(s2) m.(s3);
-  blake2_mixing wv (size 2) (size 6) (size 10) (size 14) m.(s4) m.(s5);
-  blake2_mixing wv (size 3) (size 7) (size 11) (size 15) m.(s6) m.(s7)
+  blake2_mixing p wv (size 0) (size 4) (size  8) (size 12) m.(s0) m.(s1);
+  blake2_mixing p wv (size 1) (size 5) (size  9) (size 13) m.(s2) m.(s3);
+  blake2_mixing p wv (size 2) (size 6) (size 10) (size 14) m.(s4) m.(s5);
+  blake2_mixing p wv (size 3) (size 7) (size 11) (size 15) m.(s6) m.(s7)
 
 
 #set-options "--z3rlimit 15"
 
-val blake2_round2 : wv:vector_wp -> m:block_wp -> i:size_t{size_v i <= 9} ->
+val blake2_round2 : p: alg -> wv:vector_wp p -> m:block_wp p -> i:size_t{size_v i <= 9} ->
   Stack unit
     (requires (fun h -> live h wv /\ live h m
                   /\ disjoint wv m))
     (ensures  (fun h0 _ h1 -> modifies1 wv h0 h1
-                         /\ h1.[wv] == Spec.blake2_round2 Spec.Blake2S h0.[wv] h0.[m] (v i)))
+                         /\ h1.[wv] == Spec.blake2_round2 p h0.[wv] h0.[m] (v i)))
 
 [@ Substitute ]
-let blake2_round2 wv m i =
+let blake2_round2 p wv m i =
   let start_idx = (i %. (size 10)) *. (size 16) in
   let s8 = get_sigma_sub start_idx (size 8) in
   let s9 = get_sigma_sub start_idx (size 9) in
@@ -221,49 +229,50 @@ let blake2_round2 wv m i =
   let s13 = get_sigma_sub start_idx (size 13) in
   let s14 = get_sigma_sub start_idx (size 14) in
   let s15 = get_sigma_sub start_idx (size 15) in
-  blake2_mixing wv (size 0) (size 5) (size 10) (size 15) m.(s8) m.(s9);
-  blake2_mixing wv (size 1) (size 6) (size 11) (size 12) m.(s10) m.(s11);
-  blake2_mixing wv (size 2) (size 7) (size  8) (size 13) m.(s12) m.(s13);
-  blake2_mixing wv (size 3) (size 4) (size  9) (size 14) m.(s14) m.(s15)
+  blake2_mixing p wv (size 0) (size 5) (size 10) (size 15) m.(s8) m.(s9);
+  blake2_mixing p wv (size 1) (size 6) (size 11) (size 12) m.(s10) m.(s11);
+  blake2_mixing p wv (size 2) (size 7) (size  8) (size 13) m.(s12) m.(s13);
+  blake2_mixing p wv (size 3) (size 4) (size  9) (size 14) m.(s14) m.(s15)
 
 
 #reset-options
 
-val blake2_round : wv:vector_wp -> m:block_wp -> i:size_t{v i <= 9} ->
+val blake2_round : p:alg -> wv:vector_wp p -> m:block_wp p -> i:size_t{v i <= 9} ->
   Stack unit
     (requires (fun h -> live h wv /\ live h m
                    /\ disjoint wv m))
     (ensures  (fun h0 _ h1 -> modifies1 wv h0 h1
-                         /\ h1.[wv] == Spec.blake2_round Spec.Blake2S h0.[m] (v i) h0.[wv]))
+                         /\ h1.[wv] == Spec.blake2_round p h0.[m] (v i) h0.[wv]))
 
-let blake2_round wv m i =
-  blake2_round1 wv m i;
-  blake2_round2 wv m i
+let blake2_round p wv m i =
+  blake2_round1 p wv m i;
+  blake2_round2 p wv m i
 
 
 #reset-options "--z3rlimit 15"
 
 val blake2_compress1:
-    wv:vector_wp
-  -> s:hash_wp
-  -> m:block_wp
-  -> offset:uint64
+    p:alg
+  -> wv:vector_wp p
+  -> s:hash_wp p
+  -> m:block_wp p
+  -> offset:limb_t p
   -> flag:bool ->
   Stack unit
     (requires (fun h -> live h s /\ live h m /\ live h wv
                      /\ disjoint wv s /\ disjoint wv m))
     (ensures  (fun h0 _ h1 -> modifies1 wv h0 h1
-                         /\ h1.[wv] == Spec.blake2_compress1 Spec.Blake2S h0.[wv] h0.[s] h0.[m] offset flag))
+                         /\ h1.[wv] == Spec.blake2_compress1 p h0.[wv] h0.[s] h0.[m] offset flag))
 
 [@ Substitute ]
-let blake2_compress1 wv s m offset flag =
+let blake2_compress1 p wv s m offset flag =
   update_sub wv (size 0) (size 8) s;
-  set_iv_sub wv;
-  let low_offset = Spec.limb_to_word Spec.Blake2S offset in
-  let high_offset = Spec.limb_to_word Spec.Blake2S (offset >>. size 32) in
+  set_iv_sub p wv;
+  let low_offset = Spec.limb_to_word p offset in
+  let high_offset = Spec.limb_to_word p (offset >>. size 32) in
   let wv_12 = logxor wv.(size 12) low_offset in
   let wv_13 = logxor wv.(size 13) high_offset in
-  let wv_14 = logxor wv.(size 14) (ones (Spec.wt Spec.Blake2S) SEC) in
+  let wv_14 = logxor wv.(size 14) (ones (Spec.wt p) SEC) in
   wv.(size 12) <- wv_12;
   wv.(size 13) <- wv_13;
  (if flag then wv.(size 14) <- wv_14)
@@ -272,226 +281,236 @@ let blake2_compress1 wv s m offset flag =
 #reset-options "--z3rlimit 25"
 
 val blake2_compress2 :
-    wv:vector_wp
-  -> m:block_wp ->
+    p: alg
+  -> wv:vector_wp p
+  -> m:block_wp p ->
   Stack unit
     (requires (fun h -> live h wv /\ live h m /\ disjoint wv m))
     (ensures  (fun h0 _ h1 -> modifies1 wv h0 h1
-                         /\ h1.[wv] == Spec.blake2_compress2 Spec.Blake2S h0.[wv] h0.[m]))
+                         /\ h1.[wv] == Spec.blake2_compress2 p h0.[wv] h0.[m]))
 
 [@ Substitute ]
-let blake2_compress2 wv m =
+let blake2_compress2 p wv m =
   let h0 = ST.get () in
   [@inline_let]
-  let spec h = Spec.blake2_round Spec.Blake2S h.[m] in
-  loop1 h0 (size (Spec.rounds Spec.Blake2S)) wv spec
+  let spec h = Spec.blake2_round p h.[m] in
+  loop1 h0 (size (Spec.rounds p)) wv spec
   (fun i ->
-    Loops.unfold_repeati (Spec.rounds Spec.Blake2S) (spec h0) (as_seq h0 wv) (v i);
-    blake2_round wv m i)
+    Loops.unfold_repeati (Spec.rounds p) (spec h0) (as_seq h0 wv) (v i);
+    blake2_round p wv m i)
 
 
 #reset-options "--z3rlimit 15"
 
 val blake2_compress3_inner :
-    wv:vector_wp
+    p:alg
+  -> wv:vector_wp p
   -> i:size_t{size_v i < 8}
-  -> s:hash_wp ->
+  -> s:hash_wp p ->
   Stack unit
     (requires (fun h -> live h s /\ live h wv
                    /\ disjoint s wv /\ disjoint wv s))
     (ensures  (fun h0 _ h1 -> modifies1 s h0 h1
-                         /\ h1.[s] == Spec.blake2_compress3_inner Spec.Blake2S h0.[wv] (v i) h0.[s]))
+                         /\ h1.[s] == Spec.blake2_compress3_inner p h0.[wv] (v i) h0.[s]))
 
 [@ Substitute ]
-let blake2_compress3_inner wv i s =
+let blake2_compress3_inner p wv i s =
   let i_plus_8 = i +. (size 8) in
   let hi_xor_wvi = s.(i) ^. wv.(i) in
-  let hi = logxor #U32 hi_xor_wvi wv.(i_plus_8) in
+  let hi = logxor #(Spec.wt p) hi_xor_wvi wv.(i_plus_8) in
   s.(i) <- hi
 
 
 #reset-options "--z3rlimit 25"
 
 val blake2_compress3 :
-    wv:vector_wp
-  -> s:hash_wp ->
+    p:alg
+  -> wv:vector_wp p
+  -> s:hash_wp p ->
   Stack unit
     (requires (fun h -> live h s /\ live h wv
                      /\ disjoint wv s /\ disjoint s wv))
     (ensures  (fun h0 _ h1 -> modifies1 s h0 h1
-                         /\ h1.[s] == Spec.blake2_compress3 Spec.Blake2S h0.[wv] h0.[s]))
+                         /\ h1.[s] == Spec.blake2_compress3 p h0.[wv] h0.[s]))
 
 [@ Substitute ]
-let blake2_compress3 wv s =
+let blake2_compress3 p wv s =
   [@inline_let]
-  let spec h = Spec.blake2_compress3_inner Spec.Blake2S h.[wv] in
+  let spec h = Spec.blake2_compress3_inner p h.[wv] in
   let h0 = ST.get () in
   loop1 h0 (size 8) s
     (fun h -> spec h)
     (fun i ->
       Loops.unfold_repeati 8 (spec h0) (as_seq h0 s) (v i);
-      blake2_compress3_inner wv i s)
+      blake2_compress3_inner p wv i s)
 
 
 #reset-options "--z3rlimit 15"
 
 val blake2_compress :
-    s:hash_wp
-  -> m:block_wp
-  -> offset:uint64
+    p:alg
+  -> s:hash_wp p
+  -> m:block_wp p
+  -> offset:limb_t p
   -> flag:bool ->
   Stack unit
     (requires (fun h -> live h s /\ live h m
                      /\ disjoint s m /\ disjoint m s))
     (ensures  (fun h0 _ h1 -> modifies1 s h0 h1
-                         /\ h1.[s] == Spec.blake2_compress Spec.Blake2S h0.[s] h0.[m] offset flag))
+                         /\ h1.[s] == Spec.blake2_compress p h0.[s] h0.[m] offset flag))
 
-let blake2_compress s m offset flag =
+let blake2_compress p s m offset flag =
   let h0 = ST.get () in
   [@inline_let]
-  let spec _ h1 = h1.[s] == Spec.blake2_compress Spec.Blake2S h0.[s] h0.[m] offset flag in
+  let spec _ h1 = h1.[s] == Spec.blake2_compress p h0.[s] h0.[m] offset flag in
   salloc1_trivial h0 (size 16) (u32 0) (Ghost.hide (LowStar.Buffer.loc_buffer s)) spec
   (fun wv ->
-    blake2_compress1 wv s m offset flag;
-    blake2_compress2 wv m;
-    blake2_compress3 wv s)
+    blake2_compress1 p wv s m offset flag;
+    blake2_compress2 p wv m;
+    blake2_compress3 p wv s)
 
 
 #reset-options "--z3rlimit 15"
 
-val blake2s_update_block:
-    hash:hash_wp
-  -> prev:uint64
-  -> d:block_p ->
+val blake2_update_block:
+    p: alg
+  -> hash:hash_wp p
+  -> prev:limb_t p
+  -> d:block_p p ->
   Stack unit
     (requires (fun h -> live h hash /\ live h d /\ disjoint hash d))
     (ensures  (fun h0 _ h1 -> modifies1 hash h0 h1
-                         /\ h1.[hash] == Spec.blake2_update_block Spec.Blake2S (uint_v prev) h0.[d] h0.[hash]))
+                         /\ h1.[hash] == Spec.blake2_update_block p (uint_v prev) h0.[d] h0.[hash]))
 
-let blake2s_update_block hash prev d =
+let blake2_update_block p hash prev d =
   let h0 = ST.get () in
   [@inline_let]
-  let spec _ h1 = h1.[hash] == Spec.blake2_update_block Spec.Blake2S (uint_v prev) h0.[d] h0.[hash] in
+  let spec _ h1 = h1.[hash] == Spec.blake2_update_block p (uint_v prev) h0.[d] h0.[hash] in
   salloc1_trivial h0 (size 16) (u32 0) (Ghost.hide (LowStar.Buffer.loc_buffer hash)) spec
   (fun block_w ->
      uints_from_bytes_le block_w (size Spec.size_block_w) d;
      let offset = prev in
-     blake2_compress hash block_w offset false)
+     blake2_compress p hash block_w offset false)
 
 
 #reset-options
 
-val blake2s_init_hash:
-    hash:hash_wp
+val blake2_init_hash:
+    p:alg
+  -> hash:hash_wp p
   -> kk:size_t{v kk <= 32}
-  -> nn:size_t{1 <= v nn /\ v nn <= 32} ->
+  -> nn:size_t{1 <= v nn /\ v nn <= Spec.max_output p} ->
   Stack unit
      (requires (fun h -> live h hash))
      (ensures  (fun h0 _ h1 -> modifies1 hash h0 h1
-                          /\ h1.[hash] == Spec.blake2_init_hash Spec.Blake2S (v kk) (v nn)))
+                          /\ h1.[hash] == Spec.blake2_init_hash p (v kk) (v nn)))
 [@ Substitute]
-let blake2s_init_hash hash kk nn =
-  set_iv hash;
+let blake2_init_hash p hash kk nn =
+  set_iv p hash;
   let s0 = hash.(size 0) in
   let kk_shift_8 = shift_left #U32 (size_to_uint32 kk) (size 8) in
-  let s0' = s0 ^. (u32 0x01010000) ^. kk_shift_8 ^. size_to_uint32 nn in
+  let s0' = s0 ^. (Spec.nat_to_word p 0x01010000) ^. kk_shift_8 ^. size_to_uint32 nn in
   hash.(size 0) <- s0'
 
 
 #reset-options "--z3rlimit 15"
 
-val blake2s_init_branching:
+val blake2_init_branching:
     #vkk:size_t
-  -> hash:hash_wp
+  -> p:alg
+  -> hash:hash_wp p
   -> key_block:lbuffer uint8 64
   -> k:lbuffer uint8 (v vkk)
   -> kk:size_t{v kk <= 32 /\ kk == vkk}
-  -> nn:size_t{1 <= v nn /\ v nn <= 32} ->
+  -> nn:size_t{1 <= v nn /\ v nn <= Spec.max_output p} ->
   Stack unit
     (requires (fun h -> live h hash /\ live h k /\ live h key_block
                    /\ disjoint hash k /\ disjoint hash key_block /\ disjoint key_block k))
     (ensures  (fun h0 _ h1 -> modifies2 hash key_block h0 h1
                     /\ (if (v kk) = 0 then h1.[hash] == h0.[hash] else
                        let key_block1 = Seq.update_sub #uint8 #64 h0.[key_block] 0 (v kk) h0.[k] in
-                       h1.[hash] == Spec.blake2_update_block Spec.Blake2S (Spec.size_block Spec.Blake2S) key_block1 h0.[hash])))
+                       h1.[hash] == Spec.blake2_update_block p (Spec.size_block p) key_block1 h0.[hash])))
 
 [@ Substitute ]
-let blake2s_init_branching #vkk hash key_block k kk nn =
+let blake2_init_branching #vkk p hash key_block k kk nn =
   let h0 = ST.get () in
   if kk <>. (size 0) then
   begin
     update_sub key_block (size 0) kk k;
-    let prev = Spec.word_to_limb Spec.Blake2S (secret (size_block Spec.Blake2S)) in
-    blake2s_update_block hash prev key_block
+    let prev = Spec.word_to_limb p (secret (size_block p)) in
+    blake2_update_block p hash prev key_block
   end
 
 
 #reset-options "--z3rlimit 15"
 
-val blake2s_init:
+val blake2_init:
     #vkk:size_t
-  -> hash:hash_wp
+  -> p:alg
+  -> hash:hash_wp p
   -> k:lbuffer uint8 (v vkk)
   -> kk:size_t{v kk <= 32 /\ kk == vkk}
-  -> nn:size_t{1 <= v nn /\ v nn <= 32} ->
+  -> nn:size_t{1 <= v nn /\ v nn <= Spec.max_output p} ->
   Stack unit
     (requires (fun h -> live h hash
                    /\ live h k
                    /\ disjoint hash k /\ disjoint k hash))
     (ensures  (fun h0 _ h1 -> modifies1 hash h0 h1
-                         /\ h1.[hash] == Spec.Blake2.blake2_init Spec.Blake2S (v kk) h0.[k] (v nn)))
+                         /\ h1.[hash] == Spec.Blake2.blake2_init p (v kk) h0.[k] (v nn)))
 
 [@ Substitute ]
-let blake2s_init #vkk hash k kk nn =
+let blake2_init #vkk p hash k kk nn =
   let h0 = ST.get () in
   salloc1_trivial h0 (size 64) (u8 0) (Ghost.hide (LowStar.Buffer.loc_buffer hash))
-  (fun _ h1 -> h1.[hash] == Spec.blake2_init Spec.Blake2S (size_v kk) h0.[k] (v nn))
+  (fun _ h1 -> h1.[hash] == Spec.blake2_init p (size_v kk) h0.[k] (v nn))
   (fun key_block ->
-    blake2s_init_hash hash kk nn;
-    blake2s_init_branching #vkk hash key_block k kk nn)
+    blake2_init_hash p hash kk nn;
+    blake2_init_branching #vkk p hash key_block k kk nn)
 
 
 #reset-options "--z3rlimit 15"
 
-val blake2s_update_last:
+val blake2_update_last:
     #vlen: size_t
-  -> hash: hash_wp
-  -> prev: uint64
+  -> p: alg
+  -> hash: hash_wp p
+  -> prev: limb_t p
   -> last: lbuffer uint8 (v vlen)
-  -> len: size_t{v len <= Spec.size_block Spec.Blake2S /\ len == vlen} ->
+  -> len: size_t{v len <= Spec.size_block p /\ len == vlen} ->
   Stack unit
     (requires (fun h -> live h hash /\ live h last /\ disjoint hash last))
     (ensures  (fun h0 _ h1 -> modifies1 hash h0 h1
-                         /\ h1.[hash] == Spec.Blake2.blake2_update_last Spec.Blake2S (uint_v prev) (v len) h0.[last] h0.[hash]))
+                         /\ h1.[hash] == Spec.Blake2.blake2_update_last p (uint_v prev) (v len) h0.[last] h0.[hash]))
 
-let blake2s_update_last #vlen hash prev last len =
+let blake2_update_last #vlen p hash prev last len =
   push_frame ();
-  let last_block = create #uint8 64ul (u8 0) in
-  let last_block_w = create #uint32 16ul (u32 0) in
-  update_sub last_block (size 0) len last;
-  uints_from_bytes_le last_block_w (size 16) last_block;
+  let last_block = create #uint8 (size 64) (u8 0) in
+  let last_block_w = create #(word_t p) (size 16) (Spec.nat_to_word p 0) in
+  update_sub #(word_t p) #16 #(v vlen) last_block (size 0) len last;
+  uints_from_bytes_le #(Spec.wt p) #SEC #16 last_block_w (size 16) last_block;
   let offset = prev in
-  blake2_compress hash last_block_w offset true;
+  blake2_compress p hash last_block_w offset true;
   pop_frame ()
 
 
 #reset-options "--z3rlimit 15"
 
-val blake2s_finish:
+val blake2_finish:
     #vnn: size_t
+  -> p: alg
   -> output: lbuffer uint8 (v vnn)
-  -> hash: hash_wp
+  -> hash: hash_wp p
   -> nn: size_t{1 <= v nn /\ v nn <= 32 /\ nn == vnn} ->
   Stack unit
     (requires (fun h -> live h hash
                    /\ live h output /\ disjoint output hash /\ disjoint hash output))
     (ensures  (fun h0 _ h1 -> modifies1 output h0 h1
-                         /\ h1.[output] == Spec.Blake2.blake2_finish Spec.Blake2S h0.[hash] (v nn)))
+                         /\ h1.[output] == Spec.Blake2.blake2_finish p h0.[hash] (v nn)))
 
-let blake2s_finish #vnn output hash nn =
+let blake2_finish #vnn p output hash nn =
   let h0 = ST.get () in
   salloc1_trivial h0 (size 32) (u8 0) (Ghost.hide (LowStar.Buffer.loc_buffer output))
-  (fun _ h1 -> h1.[output] == Spec.Blake2.blake2_finish Spec.Blake2S h0.[hash] (v nn))
+  (fun _ h1 -> h1.[output] == Spec.Blake2.blake2_finish p h0.[hash] (v nn))
   (fun full ->
     uints_to_bytes_le full (size 8) hash;
     let final = sub full (size 0) nn in
@@ -501,55 +520,56 @@ let blake2s_finish #vnn output hash nn =
 #reset-options "--z3rlimit 50"
 
 noextract inline_for_extraction
-let spec_prev1 (klen:size_nat{klen == 0 \/ klen == 1})
-	      (dlen:size_nat{if klen = 0 then dlen < pow2 64 else dlen + 64 < pow2 64})
-	      (i:size_nat{i < dlen/64}) : r:nat{r < pow2 64} = (klen + i + 1) * 64
+let spec_prev1 (p:alg) (klen:size_nat{klen == 0 \/ klen == 1})
+	      (dlen:size_nat{if klen = 0 then dlen < Spec.max_limb p else dlen + Spec.size_block p < Spec.max_limb p})
+	      (i:size_nat{i < dlen / (Spec.size_block p)}) : r:nat{r < Spec.max_limb p} = (klen + i + 1) * Spec.size_block p
 
 noextract inline_for_extraction
-let spec_prev2 (klen:size_nat{klen == 0 \/ klen == 1})
-	      (dlen:size_nat{if klen = 0 then dlen < pow2 64 else dlen + 64 < pow2 64})
-	      (i:size_nat{i == dlen/64}) : r:nat{r < pow2 64} = (klen * 64) + dlen
+let spec_prev2 (p:alg) (klen:size_nat{klen == 0 \/ klen == 1})
+	      (dlen:size_nat{if klen = 0 then dlen < Spec.max_limb p else dlen + Spec.size_block p < Spec.max_limb p})
+	      (i:size_nat{i == dlen / (Spec.size_block p)}) : r:nat{r < Spec.max_limb p} = (klen * (Spec.size_block p)) + dlen
 
 
 noextract inline_for_extraction
-let prev1 (klen:size_t{v klen == 0 \/ v klen == 1})
-          (dlen:size_t{if v klen = 0 then v dlen < pow2 64 else v dlen + 64 < pow2 64})
-	  (i:size_t{v i < v dlen/64}) :
-	  (prev:uint64{uint_v prev == spec_prev1 (v klen) (v dlen) (v i)})
-	  = let p = to_u64 (klen +. i +. size 1) *. u64 64 in
-	    assert (uint_v p == spec_prev1 (v klen) (v dlen) (v i));
+let prev1 (p:alg) (klen:size_t{v klen == 0 \/ v klen == 1})
+          (dlen:size_t{if v klen = 0 then v dlen < Spec.max_limb p else v dlen + Spec.size_block p < Spec.max_limb p})
+	  (i:size_t{v i < v dlen / (Spec.size_block p)}) :
+	  (prev:uint64{uint_v prev == spec_prev1 p (v klen) (v dlen) (v i)})
+	  = let p = Spec.Blake2.word_to_limb p (klen +. i +. size 1) *. Spec.nat_to_limb p 64 in
+	    assert (uint_v p == spec_prev1 p (v klen) (v dlen) (v i));
 	    p
 
 noextract inline_for_extraction
-let prev2 (klen:size_t{v klen == 0 \/ v klen == 1})
-          (dlen:size_t{if v klen = 0 then v dlen < pow2 64 else v dlen + 64 < pow2 64})
-	  (i:size_t{v i == v dlen/64}) :
-	  (prev:uint64{uint_v prev == spec_prev2 (v klen) (v dlen) (v i)})
-	  = to_u64 dlen +. to_u64 (klen *. size 64)
+let prev2 (p:alg) (klen:size_t{v klen == 0 \/ v klen == 1})
+          (dlen:size_t{if v klen = 0 then v dlen < Spec.max_limb p else v dlen + Spec.size_block p < Spec.max_limb p})
+	  (i:size_t{v i == v dlen / (Spec.size_block p)}) :
+	  (prev:uint64{uint_v prev == spec_prev2 p (v klen) (v dlen) (v i)})
+	  = Spec.word_to_limb p dlen +. Spec.word_to_limb p (klen *. size 64)
 
 
 #reset-options "--z3rlimit 150"
 
 inline_for_extraction
-val blake2s_update:
+val blake2_update:
     #vll: size_t
-  -> hash: hash_wp
+  -> p: alg
+  -> hash: hash_wp p
   -> d: lbuffer uint8 (v vll)
   -> ll: size_t{v ll == v vll}
-  -> kk: size_t{v kk <= 32 /\ (if v kk = 0 then v ll < pow2 64 else v ll + 64 < pow2 64)} ->
+  -> kk: size_t{v kk <= 32 /\ (if v kk = 0 then v ll < Spec.max_limb p else v ll + Spec.size_block p < Spec.max_limb p)} ->
   Stack unit
     (requires (fun h -> live h hash /\ live h d /\ disjoint hash d))
     (ensures  (fun h0 _ h1 -> modifies1 hash h0 h1
-                         /\ h1.[hash] == Spec.blake2_update Spec.Blake2S h0.[hash] h0.[d] (v kk)))
+                         /\ h1.[hash] == Spec.blake2_update p h0.[hash] h0.[d] (v kk)))
 
-let blake2s_update #vll hash d ll kk =
+let blake2_update #vll p hash d ll kk =
   let h0 = ST.get() in
   let klen = if kk =. size 0 then size 0 else size 1 in
-  loopi_blocks (size_block Spec.Blake2S) ll d
-    (Spec.spec_update_block Spec.Blake2S ((v klen + 1) * (Spec.size_block Spec.Blake2S)))
-    (Spec.spec_update_last Spec.Blake2S (v klen * (Spec.size_block Spec.Blake2S) + v ll))
-    (fun i block hash -> blake2s_update_block hash (prev1 klen ll i) block)
-    (fun i len last hash -> blake2s_update_last #(ll %. size (Spec.size_block Spec.Blake2S)) hash (prev2 klen ll i) last len)
+  loopi_blocks (size_block p) ll d
+    (Spec.spec_update_block p ((v klen + 1) * (Spec.size_block p)))
+    (Spec.spec_update_last p (v klen * (Spec.size_block p) + v ll))
+    (fun i block hash -> blake2_update_block p hash (prev1 p klen ll i) block)
+    (fun i len last hash -> blake2_update_last #(ll %. size (Spec.size_block p)) p hash (prev2 klen ll i) last len)
     hash
 
 
@@ -576,6 +596,6 @@ let blake2s output d ll k kk nn =
   salloc1_trivial h0 (size 8) (u32 0) (Ghost.hide (LowStar.Buffer.loc_buffer output))
   (fun _ h1 -> h1.[output] == Spec.Blake2.blake2s h0.[d] (v kk) h0.[k] (v nn))
   (fun hash ->
-    blake2s_init #kk hash k kk nn;
-    blake2s_update #ll hash d ll kk;
-    blake2s_finish #nn output hash nn)
+    blake2_init #kk Spec.Blake2S hash k kk nn;
+    blake2_update #ll Spec.Blake2S hash d ll kk;
+    blake2_finish #nn Spec.Blake2S output hash nn)
