lib/fst/Lib.Buffer.fst
@@ -83,23 +83,23 @@ let icopy #a #len o clen i =
 let memset #a #blen b init len =
   B.fill #a b init len
 
-let update_sub #a #len dst start n src =
+let update_sub #a #dlen #slen dst start n src =
   let h0 = ST.get () in
   LowStar.BufferOps.blit src 0ul dst (size_to_UInt32 start) (size_to_UInt32 n);
   let h1 = ST.get () in
   assert (forall (k:nat{k < v n}). bget h1 dst (v start + k) == bget h0 src k);
   FStar.Seq.lemma_eq_intro
     (B.as_seq h1 dst)
-    (Seq.update_sub #a #len (B.as_seq h0 dst) (v start) (v n) (B.as_seq h0 src))
+    (Seq.update_sub #a #dlen (B.as_seq h0 dst) (v start) (v n) (B.as_seq h0 src))
 
-let update_isub #a #len dst start n src =
+let update_isub #a #dlen #slen dst start n src =
   let h0 = ST.get () in
   LowStar.BufferOps.blit src 0ul dst (size_to_UInt32 start) (size_to_UInt32 n);
   let h1 = ST.get () in
   assert (forall (k:nat{k < v n}). bget h1 dst (v start + k) == ibget h0 src k);
   FStar.Seq.lemma_eq_intro
     (B.as_seq h1 dst)
-    (Seq.update_sub #a #len (B.as_seq h0 dst) (v start) (v n) (IB.as_seq h0 src))
+    (Seq.update_sub #a #dlen (B.as_seq h0 dst) (v start) (v n) (IB.as_seq h0 src))
 
 let update_sub_f #a #len h0 buf start n spec f =
   let h0 = ST.get () in
