specs/Spec.Blake2.fst
@@ -34,6 +34,12 @@ inline_for_extraction let size_block (a:alg) : size_nat = size_block_w * (size_w
 inline_for_extraction let size_const_iv : size_nat = 8
 inline_for_extraction let size_const_sigma : size_nat = 160
 
+inline_for_extraction
+let max_output (a:alg) =
+  match a with
+  | Blake2S -> 32
+  | Blake2B -> 64
+
 
 (* Definition of base types *)
 inline_for_extraction
@@ -346,7 +352,7 @@ let blake2_update_block a prev d s =
 val blake2_init_hash:
     a:alg
   -> kk:size_nat{kk <= 32}
-  -> nn:size_nat{1 <= nn /\ nn <= 32} ->
+  -> nn:size_nat{1 <= nn /\ nn <= max_output a} ->
   Tot (hash_ws a)
 
 let blake2_init_hash a kk nn =
@@ -359,7 +365,7 @@ val blake2_init:
     a:alg
   -> kk:size_nat{kk <= 32}
   -> k:lbytes kk
-  -> nn:size_nat{1 <= nn /\ nn <= 32} ->
+  -> nn:size_nat{1 <= nn /\ nn <= max_output a} ->
   Tot (hash_ws a)
 
 let blake2_init a kk k nn =
@@ -393,22 +399,22 @@ val blake2_update:
   -> kk:size_nat{kk <= 32 /\ (if kk = 0 then length d <= max_limb a else length d + (size_block a) <= max_limb a)} ->
   Tot (hash_ws a)
 
-let spec_update_block 
-    (a:alg) 
-    (init:nat) 
+let spec_update_block
+    (a:alg)
+    (init:nat)
     (i:nat{init + (i * size_block a) <= max_limb a}) =
     blake2_update_block a (init + (i * size_block a))
 
-let spec_update_last 
-    (a:alg) 
+let spec_update_last
+    (a:alg)
     (len:nat{len <= max_limb a})
     (i:nat) =
-    blake2_update_last a len 
-    
+    blake2_update_last a len
+
 let blake2_update a s d kk =
   let ll = length d in
   let klen = if kk = 0 then 0 else 1 in
-  repeati_blocks (size_block a) d 
+  repeati_blocks (size_block a) d
     (spec_update_block a ((klen + 1) * size_block a))
     (spec_update_last a (klen * (size_block a) + ll))
     s
@@ -417,7 +423,7 @@ let blake2_update a s d kk =
 val blake2_finish:
     a:alg
   -> s:hash_ws a
-  -> nn:size_nat{1 <= nn /\ nn <= 32} ->
+  -> nn:size_nat{1 <= nn /\ nn <= max_output a} ->
   Tot (lbytes nn)
 
 let blake2_finish a s nn =
@@ -430,7 +436,7 @@ val blake2:
   -> d:bytes
   -> kk:size_nat{kk <= 32 /\ (if kk = 0 then length d <= max_limb a else length d + (size_block a) <= max_limb a)}
   -> k:lbytes kk
-  -> nn:size_nat{1 <= nn /\ nn <= 32} ->
+  -> nn:size_nat{1 <= nn /\ nn <= max_output a} ->
   Tot (lbytes nn)
 
 let blake2 a d kk k nn =
@@ -453,7 +459,7 @@ val blake2b:
     d:bytes
   -> kk:size_nat{kk <= 32 /\ (if kk = 0 then length d < pow2 128 else length d + 128  < pow2 128)}
   -> k:lbytes kk
-  -> nn:size_nat{1 <= nn /\ nn <= 32} ->
+  -> nn:size_nat{1 <= nn /\ nn <= 64} ->
   Tot (lbytes nn)
 
 let blake2b d kk k n = blake2 Blake2B d kk k n
